AutoKchp/Internal/TotalOrder.lean
@@ -1,5 +1,10 @@
-module
+/-
+Copyright (c) 2026 Marc Perlade. All rights reserved.
+Released under Apache 2.0 license as described in the file LICENSE.
+Authors: Marc Perlade
+-/
 
+module
 
 public section
 
@@ -16,7 +21,7 @@ class TotalOrd α extends LE α where
 
 instance [t: TotalOrd α]: DecidableLE α := t.le_decidable
 instance [t: TotalOrd α]: DecidableEq α := t.eq_decidable
-instance [t: TotalOrd α]: LT α := ⟨fun x y => x ≤ y ∧ x ≠ y⟩
+instance (priority := high) [t: TotalOrd α]: LT α := ⟨fun x y => x ≤ y ∧ x ≠ y⟩
 instance [t: TotalOrd α]: DecidableLT α := fun _ _ => instDecidableAnd
 
 
@@ -25,5 +30,15 @@ theorem TotalOrd.lt_trans [t: TotalOrd α] {a b c: α} (h1: a < b) (h2: b < c): 
     t.le_trans h1.left h2.left,
     fun eq => h1.right (t.le_antisymm h1.left (eq ▸ h2.left))
   ⟩
+
+
+instance {n: Nat}: TotalOrd (Fin n) := {
+  le_decidable := inferInstance
+  eq_decidable := inferInstance
+  le_refl := Fin.le_refl
+  le_trans := Fin.le_trans
+  le_antisymm := Fin.le_antisymm
+  le_total := Fin.le_total
+}
 
 end
